---
title: "Ecuaciones"
author: "Daniel"
date: "20-01-2020"
output: ioslides_presentation
---

```{r setup, include=FALSE}
knitr::opts_chunk$set(echo = FALSE)
```

## Regresión Lineal

$$y = \beta _0+\beta_1x$$
$$h(x) = \theta_0+\theta_1x$$
$$J(\theta_0, \theta_1)= \frac{1}{2m}\sum_{i=1}^{m}(h(x)-y)^2$$

## Regresión Lineal 2
repetir hasta converger{
$$\theta_j = \theta_j-\alpha\cdot \frac{\partial}{\partial \theta_j}J(\theta_0, \theta_1)\thinspace \thinspace \thinspace \forall \thinspace  j=0 \thinspace \thinspace  and \thinspace  \thinspace  j =1$$
}


## Regresión Lineal 3

repetir hasta converger{
$$\theta_j = \theta_j-\alpha\cdot \frac{\partial}{\partial \theta_j}\sum_{i=1}^{m}(h(x^{(i)})-y^{(i)})$$

$$\theta_j = \theta_j-\alpha\cdot \frac{\partial}{\partial \theta_j}\sum_{i=1}^{m}(h(x^{(i)})-y^{(i)})x^{(i)}$$
}

## Regresión Lineal 4

$$x_{stand} = \frac{x_j-\mu_j}{\sigma_j}$$

## Regresión Logística 1

$$Y_i = \left\{\begin{array}\\ 1: \mbox{Evento exitoso}\\0: \mbox{en caso contrario} \end{array}\right.$$

$$P_i = Pr(Y_i = 1) = P(X_i,\theta)$$
$$Q_i = Pr(Y_i = 0) = 1-P(X_i,\theta) = Q(X_i,\theta)$$

$$odds = \frac{P}{1-P}$$
$$P = \theta_0+\theta_1x$$

## Regresión logística 2

$$logit(p) = ln(odds) =  ln(\frac{p}{1-p})$$
$$logit(p)=\theta_0\cdot x_0+\theta_1\cdot x_1+...+\theta_m\cdot x_m = \sum_{i=0}^{m}{\theta_ix_i} = \theta^{T}\cdot x $$

$$\phi(z) = \frac{1}{1-e^{-z}}$$

$$z= \theta_0\cdot x_0+\theta_1\cdot x_1+...+\theta_m\cdot x_m = \sum_{i=0}^{m}{\theta_ix_i} = \theta^{T}\cdot x$$

$$h_\theta(x)= \phi(\theta^{T}x)$$

## Regresión logística 3

$$h_\theta(x)\geq0.5$$

$$h_\theta(x)<0.5$$

$$Cost(h_{\theta}(x),y) = \left\{\begin{array}\\ -\log(h_{\theta}(x))  &   \mbox{si y = 1}\\-\log(1-h_{\theta}(x)) & \mbox{si y = 0} \end{array}\right.$$

$$J(\theta) =\frac{1}{m}\sum_{i=1}^{m}Cost(h_{\theta}(x),y)$$

$$J(\theta) = \frac{1}{m}[\sum_{i=1}^{m}y\log h_{\theta}(x)+(1-y)\log (1-h_{\theta}(x))]$$

## Regresión logística 4

repetir hasta converger{
$$ \theta _{j} := \theta_{j}- \alpha \sum_{i=1}^{m}(h_{\theta}(x^{i})-y^{i})\cdot x^{i}$$
}